theories/lib/pair.v
@@ -1,0 +1,52 @@
+Require Import logic.
+From iris.algebra Require Import agree frac.
+From iris.base_logic.lib Require Import wsat fancy_updates.
+From iris.base_logic.lib Require Export namespaces invariants.
+From iris.proofmode Require Import tactics.
+Set Default Proof Using "Type".
+Import uPred.
+
+Section defs.
+  Context {t: Type}.
+
+  Local Instance t_equiv: Equiv t := (=).
+
+  Definition pairM := (prodR fracR (agreeR (discreteC t))).
+
+  Class pairG (Σ: gFunctors) := pair_inG :> inG Σ pairM.
+
+  Definition to_pairM c : pairM := ((1/2)%Qp, (to_agree (c: leibnizC t))).
+
+End defs.
+
+Section rules.
+  Context `{@pairG t Σ} {γ: gname}.
+  
+  Definition own_pair (c: t) := own γ (to_pairM c).
+
+  Lemma own_pair_agree ks ks':
+   own_pair ks ∗ own_pair ks'  ⊢ ⌜ ks = ks' ⌝.
+  Proof.
+    iIntros "[Hs' Hs]".
+    rewrite /own_update.
+    iDestruct (own_valid_2 with "Hs Hs'") as "%".
+    iPureIntro. destruct H0 as [? ?]. simpl in H1.
+    by apply to_agree_comp_valid in H1.
+  Qed.
+
+  Lemma own_pair_update c1 c2 c3:
+    own_pair c1 ∗ own_pair c2 ⊢ |==> own_pair c3 ∗ own_pair c3 ∗ ⌜ c1 = c2 ⌝.
+  Proof.
+    iIntros "[Hs Hs']".
+    iDestruct (own_pair_agree with "[-]") as "%"; first iFrame.
+    inversion H0. subst.
+    rewrite /own_update.
+    iMod (own_update_2 with "Hs Hs'") as "[Hs Hs']"; last by iFrame.
+    rewrite pair_op frac_op' Qp_div_2.
+    apply cmra_update_exclusive.
+    split; simpl.
+    - by rewrite frac_op'.
+    - by apply to_agree_comp_valid.
+  Qed.
+
+End rules.
